Launchbury/ArityCorrect.thy
@@ -18,101 +18,28 @@ locale CorrectArityAnalysis = ArityAnalysis +
   assumes Aexp_Var: "Aexp (Var x) \<cdot> n = AE_singleton x \<cdot> (up \<cdot> n)"
   assumes Aexp_subst_App_Lam: "Aexp (e'[y::=x]) \<sqsubseteq> Aexp (App (Lam [y]. e') x)"
   assumes Aexp_App: "Aexp (App e x) \<cdot> n = Aexp e \<cdot>(inc\<cdot>n) \<squnion> AE_singleton x \<cdot> (up\<cdot>0)"
-  assumes Aexp_Lam: "Afix2 (asToHeap as)\<cdot>(Aexp e\<cdot>n) \<sqsubseteq> Aexp (Let as e)\<cdot>n"
+  assumes Aexp_Lam: "Afix (asToHeap as)\<cdot>(Aexp e\<cdot>n) \<sqsubseteq> Aexp (Let as e)\<cdot>n"
+  assumes Aexp_lookup_fresh: "atom v \<sharp> e \<Longrightarrow> (Aexp e\<cdot>a) v = \<bottom>"
 begin
-
-lemma Afix_bind_to_F: "Afix ((x, z) # \<Delta>) \<cdot> F = Afix (delete x \<Delta>) \<cdot> (ABind x z \<squnion> F)"
-  apply (rule cfun_eqI)
-  apply (simp add: Afix_eq)
-  by (metis (hide_lams, no_types) join_assoc join_comm)
-
-lemma Afix_duplicate_binds:
-  assumes  "cont G"
-  shows "Afix \<Gamma> \<cdot> ((\<Lambda> ae. G ae) \<squnion>  F) = Afix \<Gamma> \<cdot> ((\<Lambda> ae. Afix \<Gamma> \<cdot> ID \<cdot> (G ae)) \<squnion> F)"
-proof-
-  note cont_compose[OF assms, cont2cont, simp]
-  show ?thesis
-  apply (rule cfun_eqI)
-  unfolding Afix_eq
-  apply (rule below_antisym)
-  apply (rule fix_least_below)
-  apply (subst fix_eq) back back 
-  apply simp
-
-  apply (intro join_mono below_refl)
-  apply (subst fix_eq) back back
-  apply simp
-
-  apply (simp add: below_trans[OF  _ join_above1] below_trans[OF _ join_above2])
-
-  apply (rule fix_least_below, simp)
-  apply (intro join_below)
-
-  apply (subst fix_eq)  apply simp
-  
-  apply (subst fix_eq) back  apply simp
-  apply (simp add: below_trans[OF  _ join_above1] below_trans[OF _ join_above2])
-
-  apply (rule fix_least_below, simp)
-  apply (intro join_below)
-  apply (subst fix_eq) back apply simp
-  apply (simp add: below_trans[OF  _ join_above1] below_trans[OF _ join_above2])
-
-  apply (subst fix_eq) back apply simp
-  apply (simp add: below_trans[OF  _ join_above1] below_trans[OF _ join_above2])
-
-  apply simp
-
-  apply (subst fix_eq) back apply simp
-  apply (simp add: below_trans[OF  _ join_above1] below_trans[OF _ join_above2])
-  done
-qed
-
-lemma Afix_const_to_F: "Afix \<Gamma> \<cdot> F \<cdot> (a \<squnion> b) = Afix \<Gamma> \<cdot> (F \<squnion> (\<Lambda> _. b)) \<cdot>a"
-  unfolding Afix_eq
-  apply simp
-  by (metis (hide_lams, no_types) join_assoc join_comm)
 
 lemma Aexp'_Var: "Aexp' (Var x) \<cdot> n = AE_singleton x \<cdot> n"
   by (cases n) (simp_all add: Aexp_Var)
 
-lemma Aexp'_Lam: "Afix2 (asToHeap as)\<cdot>(Aexp' e\<cdot>n) \<sqsubseteq> Aexp' (Let as e)\<cdot>n"
+lemma Aexp'_Lam: "Afix (asToHeap as)\<cdot>(Aexp' e\<cdot>n) \<sqsubseteq> Aexp' (Let as e)\<cdot>n"
   by (cases n) (simp_all add: Aexp_Lam)
 
-lemma AFix_above_arg: "ae \<sqsubseteq> Afix \<Gamma> \<cdot> F \<cdot> ae"
-  apply (simp add: Aexp_Var Afix_eq ABind_def AE_singleton_def)
-  apply (subst fix_eq)
-  apply simp
-  done
-
-lemma Afix_below_var: "Afix ((x,e) # \<Gamma>) \<cdot> F \<cdot> (Aexp' e\<cdot>n) \<sqsubseteq> Afix ((x,e) # \<Gamma>)\<cdot> F \<cdot>(Aexp' (Var x)\<cdot>n)"
-proof-
-  have "(\<mu> xa. Aexp' e\<cdot>n \<squnion> (Aexp' e\<cdot>(xa x) \<squnion> (ABinds (delete x \<Gamma>)\<cdot>xa \<squnion> F\<cdot>xa))) \<sqsubseteq> (\<mu> xa. AE_singleton x \<cdot> n \<squnion> (Aexp' e\<cdot>(xa x) \<squnion> (ABinds (delete x \<Gamma>)\<cdot>xa \<squnion> F\<cdot>xa)))" (is "fix\<cdot>?F1 \<sqsubseteq> fix\<cdot>?F2")
-  proof(rule fix_least_below)
-    have F2x: "n \<sqsubseteq> (fix \<cdot> ?F2) x" by (subst fix_eq) (simp add: AE_singleton_def)
-
-    have "?F1 \<cdot> (fix \<cdot> ?F2) \<sqsubseteq> ?F2 \<cdot> (fix \<cdot> ?F2)"
-      by (auto intro: join_below simp  add: below_trans[OF _ join_above2]  below_trans[OF _ join_above1] monofun_cfun_arg F2x)
-    thus "?F1 \<cdot> (fix \<cdot> ?F2) \<sqsubseteq> (fix \<cdot> ?F2)" unfolding fix_eq[symmetric].
-  qed
-  thus ?thesis by (simp add: Aexp_Var Afix_eq ABind_def Aexp'_Var)
-qed
-  
 lemma Afix_reorder: "map_of \<Gamma> = map_of \<Delta> \<Longrightarrow> Afix \<Gamma> = Afix \<Delta>"
   by (intro cfun_eqI)(simp add: Afix_eq cong: Abinds_reorder)
 
-lemma Afix2_reorder: "map_of \<Gamma> = map_of \<Delta> \<Longrightarrow> Afix2 \<Gamma> = Afix2 \<Delta>"
-  by (intro cfun_eqI)(simp add: Afix2_eq cong: Abinds_reorder)
-
-lemma Afix2_repeat_singleton: "(\<mu> xa. Afix2 \<Gamma>\<cdot>(AE_singleton x\<cdot>(n \<squnion> xa x) \<squnion> ae)) = Afix2 \<Gamma>\<cdot>(AE_singleton x\<cdot>n \<squnion> ae)"
+lemma Afix_repeat_singleton: "(\<mu> xa. Afix \<Gamma>\<cdot>(AE_singleton x\<cdot>(n \<squnion> xa x) \<squnion> ae)) = Afix \<Gamma>\<cdot>(AE_singleton x\<cdot>n \<squnion> ae)"
   apply (rule below_antisym)
   defer
   apply (subst fix_eq, simp)
   apply (intro monofun_cfun_arg join_mono below_refl join_above1)
 
   apply (rule fix_least_below, simp)
-  apply (rule Afix2_least_below, simp)
-  apply (intro join_below below_refl iffD2[OF AE_singleton_below_iff] below_trans[OF _ fun_belowD[OF Afix2_above_arg]]  below_trans[OF _ Afix2_above_arg] join_above2)
+  apply (rule Afix_least_below, simp)
+  apply (intro join_below below_refl iffD2[OF AE_singleton_below_iff] below_trans[OF _ fun_belowD[OF Afix_above_arg]]  below_trans[OF _ Afix_above_arg] join_above2)
   apply simp
   done
 
@@ -163,17 +90,35 @@ lemma rolling_rule2:
   using rolling_rule[where g = "\<Lambda> x. G x" and f = "\<Lambda> x. F x"]
   by (auto simp add: oo_def)
 
-lemma Afix2_join_fresh: "ae' ` (domA \<Delta>) \<subseteq> {\<bottom>}  \<Longrightarrow>  Afix2 \<Delta>\<cdot>(ae \<squnion> ae') = (Afix2 \<Delta>\<cdot>ae) \<squnion> ae'"
+lemma Afix_join_fresh: "ae' ` (domA \<Delta>) \<subseteq> {\<bottom>}  \<Longrightarrow>  Afix \<Delta>\<cdot>(ae \<squnion> ae') = (Afix \<Delta>\<cdot>ae) \<squnion> ae'"
   apply (rule below_antisym)
-  apply (rule Afix2_least_below)
+  apply (rule Afix_least_below)
   apply (simp add: Abinds_join_fresh)
   apply (rule join_below)
-  apply (rule below_trans[OF Afix2_above_arg join_above1])
+  apply (rule below_trans[OF Afix_above_arg join_above1])
   apply (rule join_above2)
   apply (rule join_below[OF monofun_cfun_arg [OF join_above1]])
-  apply (rule below_trans[OF join_above2 Afix2_above_arg])
+  apply (rule below_trans[OF join_above2 Afix_above_arg])
   done
-  
+
+
+lemma Aexp'_lookup_fresh: "atom v \<sharp> e \<Longrightarrow> (Aexp' e\<cdot>a) v = \<bottom>"
+  by (cases a) (auto simp add: Aexp_lookup_fresh)
+
+lemma ABinds_lookup_fresh:
+  "atom v \<sharp> \<Gamma> \<Longrightarrow> (ABinds \<Gamma>\<cdot>ae) v = ae v"
+by (induct \<Gamma> rule: ABinds.induct) (auto simp add: fresh_Cons fresh_Pair Aexp'_lookup_fresh fresh_delete)
+
+lemma Afix_lookup_fresh:
+  assumes "atom v \<sharp> \<Gamma>"
+  shows "(Afix \<Gamma>\<cdot>ae) v = ae v"
+  apply (rule below_antisym)
+  apply (subst Afix_eq)
+  apply (rule fix_ind[where  P = "\<lambda> ae'. ae' v \<sqsubseteq> ae v"])
+  apply (auto simp add: ABinds_lookup_fresh[OF assms] fun_belowD[OF Afix_above_arg])
+  done
+
+
 lemma Abinds_append_fresh: "atom ` (domA \<Delta>) \<sharp>* \<Gamma> \<Longrightarrow>  ABinds (\<Delta> @ \<Gamma>)\<cdot>ae = ABinds \<Delta>\<cdot>(ABinds \<Gamma>\<cdot>ae)"
 proof (induct \<Delta> rule: ABinds.induct)
   case 1 thus ?case by simp
@@ -185,26 +130,73 @@ next
   from 2(1)[OF this(2)]
   have "ABinds (delete v \<Delta> @ \<Gamma>)\<cdot>ae = ABinds (delete v \<Delta>)\<cdot>(ABinds \<Gamma>\<cdot>ae)".
   moreover
-  have "delete v \<Gamma> = \<Gamma>" sorry
+  have "delete v \<Gamma> = \<Gamma>" by (metis `atom v \<sharp> \<Gamma>` delete_not_domA domA_not_fresh)
   moreover
-  have "(ABinds \<Gamma>\<cdot>ae) v = ae v" sorry
+  have "(ABinds \<Gamma>\<cdot>ae) v = ae v" by (rule ABinds_lookup_fresh[OF `atom v \<sharp> \<Gamma>`])
   ultimately
   show "ABinds (((v, e) # \<Delta>) @ \<Gamma>)\<cdot>ae = ABinds ((v, e) # \<Delta>)\<cdot>(ABinds \<Gamma>\<cdot>ae)"
     by simp
 qed  
 
+lemma Abinds_comp2join_fresh:
+  "atom ` (domA \<Delta>) \<sharp>* \<Gamma> \<Longrightarrow> ABinds \<Delta>\<cdot>(ABinds \<Gamma>\<cdot>ae) = ABinds \<Gamma> \<cdot> ae \<squnion> ABinds \<Delta>\<cdot>ae"
+proof (induct \<Delta> rule: ABinds.induct)
+  case 1 show ?case by (simp add: ABinds_above_arg del: fun_meet_simp)
+next
+  case (2 v e \<Delta>)
+  from 2(2)
+  have "atom v \<sharp> \<Gamma>" and  "atom ` domA (delete v \<Delta>) \<sharp>* \<Gamma>"
+    by (auto simp add: fresh_star_def)
+  from 2(1)[OF this(2)]
+  show ?case
+    by (simp del: fun_meet_simp add: ABinds_lookup_fresh[OF `atom v \<sharp> \<Gamma>`])
+       (metis (hide_lams, no_types) join_assoc join_comm)
+qed
 
-lemma Afix2_append_fresh:
+lemma Afix_comp2join_fresh:
+  "atom ` (domA \<Delta>) \<sharp>* \<Gamma> \<Longrightarrow> ABinds \<Delta>\<cdot>(Afix \<Gamma>\<cdot>ae) = Afix \<Gamma> \<cdot> ae \<squnion> ABinds \<Delta>\<cdot>ae"
+proof (induct \<Delta> rule: ABinds.induct)
+  case 1 show ?case by (simp add: Afix_above_arg del: fun_meet_simp)
+next
+  case (2 v e \<Delta>)
+  from 2(2)
+  have "atom v \<sharp> \<Gamma>" and  "atom ` domA (delete v \<Delta>) \<sharp>* \<Gamma>"
+    by (auto simp add: fresh_star_def)
+  from 2(1)[OF this(2)]
+  show ?case
+    by (simp del: fun_meet_simp add: Afix_lookup_fresh[OF `atom v \<sharp> \<Gamma>`])
+       (metis (hide_lams, no_types) join_assoc join_comm)
+qed
+
+lemma Afix_append_fresh:
   assumes "atom ` domA \<Delta> \<sharp>* \<Gamma>"
-  shows "Afix2 (\<Delta> @ \<Gamma>)\<cdot>ae = Afix2 \<Gamma>\<cdot>(Afix2 \<Delta>\<cdot>ae)"
-apply (rule below_antisym)
-apply (rule Afix2_least_below)
-apply (simp add:  Abinds_append_fresh[OF assms])
-sorry
+  shows "Afix (\<Delta> @ \<Gamma>)\<cdot>ae = Afix \<Gamma>\<cdot>(Afix \<Delta>\<cdot>ae)"
+proof (rule below_antisym)
+  show *: "Afix (\<Delta> @ \<Gamma>)\<cdot>ae \<sqsubseteq> Afix \<Gamma>\<cdot>(Afix \<Delta>\<cdot>ae)"
+  by (rule Afix_least_below)
+     (simp_all add:  Abinds_append_fresh[OF assms] Afix_comp2join_fresh[OF assms] Afix_above_arg below_trans[OF Afix_above_arg Afix_above_arg])
+next
+  show "Afix \<Gamma>\<cdot>(Afix \<Delta>\<cdot>ae) \<sqsubseteq> Afix (\<Delta> @ \<Gamma>)\<cdot>ae"
+  proof (rule Afix_least_below)
+    show "ABinds \<Gamma>\<cdot>(Afix (\<Delta> @ \<Gamma>)\<cdot>ae) \<sqsubseteq> Afix (\<Delta> @ \<Gamma>)\<cdot>ae"
+      apply (subst Abinds_Afix[symmetric]) back
+      apply (subst Abinds_append_fresh[OF assms])
+      apply (rule ABinds_above_arg)
+      done
+    show "Afix \<Delta>\<cdot>ae \<sqsubseteq> Afix (\<Delta> @ \<Gamma>)\<cdot>ae"
+      apply (rule Afix_least_below)
+      apply (subst Abinds_Afix[symmetric]) back
+      apply (subst Abinds_append_fresh[OF assms])
+      apply (rule monofun_cfun_arg[OF ABinds_above_arg])
+      apply (rule Afix_above_arg)
+      done
+  qed
+qed
 
-    
-lemma  "\<Gamma> : e \<Down>\<^bsub>L\<^esub> \<Delta> : v \<Longrightarrow> 
-        Afix2 \<Delta> \<cdot> (Aexp' v \<cdot> n \<squnion> ae) \<sqsubseteq> Afix2 \<Gamma> \<cdot> (Aexp' e \<cdot> n \<squnion> ae)"
+lemma  reds_improves_arity':
+       "\<Gamma> : e \<Down>\<^bsub>L\<^esub> \<Delta> : v \<Longrightarrow>
+        ae -` (-{\<bottom>}) \<subseteq> set L \<Longrightarrow> 
+        Afix \<Delta> \<cdot> (Aexp' v \<cdot> n \<squnion> ae) \<sqsubseteq> Afix \<Gamma> \<cdot> (Aexp' e \<cdot> n \<squnion> ae)"
 proof(induct arbitrary: ae n rule: reds.induct)
 case Lambda
   show ?case by simp
@@ -212,41 +204,42 @@ next
 case (Variable \<Gamma> x e L \<Delta> z ae n)
   have reorder: "map_of ((x, e) # delete x \<Gamma>) = map_of \<Gamma>" by (rule map_of_delete_insert[OF Variable.hyps(1)])
 
+  from `ae -\` (- {\<bottom>}) \<subseteq> set L`
+  have prem: "ae -` (- {\<bottom>}) \<subseteq> set (x#L)" by auto
+
   have "x \<notin> domA \<Delta>" by (rule reds_avoids_live[OF Variable(2), where x = x]) simp_all
   hence [simp]:"delete x \<Delta> = \<Delta>" by simp
 
   note IH =  Variable(3)
-  have "Afix2 ((x, z) # \<Delta>) \<cdot> (Aexp' z\<cdot>n \<squnion> ae) = (\<mu> ae'. Aexp' z\<cdot>(ae' x) \<squnion> ABinds \<Delta> \<cdot> ae' \<squnion> Aexp' z\<cdot>n \<squnion> ae)"
-    unfolding Afix2_eq by simp
+  have "Afix ((x, z) # \<Delta>) \<cdot> (Aexp' z\<cdot>n \<squnion> ae) = (\<mu> ae'. Aexp' z\<cdot>(ae' x) \<squnion> ABinds \<Delta> \<cdot> ae' \<squnion> Aexp' z\<cdot>n \<squnion> ae)"
+    unfolding Afix_eq by simp
   also have "\<dots> = (\<mu> ae'. ABinds \<Delta> \<cdot> ae' \<squnion> (Aexp' z\<cdot>n \<squnion> Aexp' z\<cdot>(ae' x) \<squnion> ae))" by (metis (hide_lams, no_types) join_assoc join_comm)
   also have "\<dots> \<sqsubseteq> (\<mu> ae'. ABinds \<Delta> \<cdot> ae' \<squnion> (Aexp' z\<cdot>(n \<squnion> ae' x) \<squnion> ae))" by (auto intro!: monofun_cfun_arg cfun_belowI join_mono[OF below_refl] join_mono[OF _ below_refl] cfun_join_below simp del: join_assoc)
-  also have "\<dots> = (\<mu> ae'. Afix2 \<Delta> \<cdot> ae' \<squnion> (Aexp' z\<cdot>(n \<squnion> ae' x) \<squnion> ae))"
+  also have "\<dots> = (\<mu> ae'. Afix \<Delta> \<cdot> ae' \<squnion> (Aexp' z\<cdot>(n \<squnion> ae' x) \<squnion> ae))"
     apply (rule fix_eq_fix)
     apply simp
     apply (subst fix_eq) back back apply simp
     apply (rule join_mono[OF _ below_refl])
     apply (rule monofun_cfun_fun)
-    apply (rule Abinds_below_Afix2)
+    apply (rule Abinds_below_Afix)
 
     apply simp
     apply (rule join_below)
-    apply (subst Afix2_eq)
+    apply (subst Afix_eq)
     apply (rule fix_least_below)
     apply simp
-    apply (rule join_below[OF _ below_refl])
     apply (subst fix_eq) back apply simp
     apply (subst fix_eq) back apply simp
     done
-  also have "\<dots> = (\<mu> ae'. Afix2 \<Delta> \<cdot> (Aexp' z\<cdot>(n \<squnion> ae' x) \<squnion> ae))"
+  also have "\<dots> = (\<mu> ae'. Afix \<Delta> \<cdot> (Aexp' z\<cdot>(n \<squnion> ae' x) \<squnion> ae))"
     apply (rule fix_eq_fix)
     apply simp
     apply (rule join_below)
-    apply (subst Afix2_eq)
+    apply (subst Afix_eq)
     apply (rule fix_least_below, simp)
-    apply (rule join_below[OF _ below_refl])
     apply (subst (1 2) fix_eq, simp)
     apply (subst fix_eq, simp)back
-    apply (rule Afix2_above_arg)
+    apply (rule Afix_above_arg)
 
     apply simp
     apply (subst fix_eq, simp) back
@@ -259,11 +252,11 @@ case (Variable \<Gamma> x e L \<Delta> z ae n)
     apply (rule below_trans[OF _ join_above2], simp)
     done
     
-  also have "\<dots> \<sqsubseteq> (\<mu> ae'. Afix2 (delete x \<Gamma>) \<cdot> (Aexp' e\<cdot>(n \<squnion> ae' x) \<squnion> ae))" by (auto intro!: monofun_cfun_arg cfun_belowI IH)
-  also have "\<dots> \<sqsubseteq> (\<mu> ae'. Afix2 ((x,e)#delete x \<Gamma>) \<cdot> (AE_singleton x \<cdot> (n \<squnion> ae' x) \<squnion> ae))"
+  also have "\<dots> \<sqsubseteq> (\<mu> ae'. Afix (delete x \<Gamma>) \<cdot> (Aexp' e\<cdot>(n \<squnion> ae' x) \<squnion> ae))" by (auto intro!: monofun_cfun_arg cfun_belowI IH[OF prem])
+  also have "\<dots> \<sqsubseteq> (\<mu> ae'. Afix ((x,e)#delete x \<Gamma>) \<cdot> (AE_singleton x \<cdot> (n \<squnion> ae' x) \<squnion> ae))"
     apply (rule monofun_cfun_arg)
     apply (rule cfun_belowI, simp)
-    apply (simp add: Afix2_eq)
+    apply (simp add: Afix_eq)
     apply (rule fix_least_below, simp)
     apply (intro join_below)
     apply (subst fix_eq, simp) back back apply (simp add: below_trans[OF _ join_above2])
@@ -280,101 +273,64 @@ case (Variable \<Gamma> x e L \<Delta> z ae n)
     apply (rule below_trans[OF _ join_above2])
     apply simp
     done
-  also have "\<dots> = Afix2 ((x,e)#delete x \<Gamma>) \<cdot> (AE_singleton x\<cdot>n \<squnion> ae)" by (rule Afix2_repeat_singleton)
-  also have "\<dots> = Afix2 ((x,e)#delete x \<Gamma>) \<cdot> (Aexp' (Var x) \<cdot> n \<squnion> ae)" by (rule arg_cong[OF Aexp'_Var[symmetric]])
-  also have "\<dots> = Afix2 \<Gamma> \<cdot> (Aexp' (Var x)\<cdot>n \<squnion> ae)" by (rule arg_cong[OF Afix2_reorder[OF reorder]])
+  also have "\<dots> = Afix ((x,e)#delete x \<Gamma>) \<cdot> (AE_singleton x\<cdot>n \<squnion> ae)" by (rule Afix_repeat_singleton)
+  also have "\<dots> = Afix ((x,e)#delete x \<Gamma>) \<cdot> (Aexp' (Var x) \<cdot> n \<squnion> ae)" by (rule arg_cong[OF Aexp'_Var[symmetric]])
+  also have "\<dots> = Afix \<Gamma> \<cdot> (Aexp' (Var x)\<cdot>n \<squnion> ae)" by (rule arg_cong[OF Afix_reorder[OF reorder]])
   finally show ?case.
 next
 case (Application y \<Gamma> e x L \<Delta> \<Theta> z e' ae n)
-  show "Afix2 \<Theta>\<cdot>(Aexp' z\<cdot>n \<squnion> ae) \<sqsubseteq> Afix2 \<Gamma>\<cdot>(Aexp' (App e x)\<cdot>n \<squnion> ae)"
+  note prem1 =  `ae -\` (- {\<bottom>}) \<subseteq> set L`
+  hence prem2: "ae -` (- {\<bottom>}) \<subseteq> set (x#L)" by auto
+  hence prem3: "(AE_singleton x\<cdot>(up\<cdot>0) \<squnion> ae) -` (- {\<bottom>}) \<subseteq> set (x#L)"  by auto
+
+  show "Afix \<Theta>\<cdot>(Aexp' z\<cdot>n \<squnion> ae) \<sqsubseteq> Afix \<Gamma>\<cdot>(Aexp' (App e x)\<cdot>n \<squnion> ae)"
   proof(cases n)
     case bottom
-    with below_trans[OF Application(5)[where n = "\<bottom>" and ae = ae, simplified ]  Application(3)[where n = "\<bottom>" and ae = ae, simplified] ]
+    with below_trans[OF Application(5)[OF prem1, where n = "\<bottom>", simplified ]  Application(3)[OF prem2, where n = "\<bottom>", simplified] ]
     show ?thesis by (simp add: lambda_strict)
   next
     case (up n')
-    note IH = Application(3)[where n = "inc\<^sub>\<bottom>\<cdot>n", unfolded up Aexp'_simps inc_bot_simps] Application(5)[where n = n, unfolded up Aexp'_simps]
-    have "Afix2 \<Theta>\<cdot>(Aexp z\<cdot>n' \<squnion> ae) \<sqsubseteq> Afix2 \<Delta>\<cdot>(Aexp e'[y::=x]\<cdot>n' \<squnion> ae)" by (rule IH)
-    also have "\<dots> \<sqsubseteq> Afix2 \<Delta>\<cdot>(Aexp (App (Lam [y]. e') x)\<cdot>n' \<squnion> ae)" by (intro monofun_cfun_arg monofun_cfun_fun Aexp_subst_App_Lam join_mono below_refl)
-    also have "\<dots> = Afix2 \<Delta>\<cdot>(Aexp (Lam [y]. e')\<cdot>(inc\<cdot>n') \<squnion> AE_singleton x \<cdot> (up\<cdot>0) \<squnion> ae)"  by (rule arg_cong[OF Aexp_App])
-    also have "\<dots> = Afix2 \<Delta>\<cdot>(Aexp (Lam [y]. e')\<cdot>(inc\<cdot>n') \<squnion> (AE_singleton x\<cdot>(up\<cdot>0) \<squnion> ae))"  by simp
-    also have "\<dots> \<sqsubseteq> Afix2 \<Gamma>\<cdot>(Aexp e\<cdot>(inc\<cdot>n') \<squnion> (AE_singleton x\<cdot>(up\<cdot>0) \<squnion> ae))" by (rule IH)
-    also have "\<dots> = Afix2 \<Gamma>\<cdot>(Aexp e\<cdot>(inc\<cdot>n') \<squnion> AE_singleton x\<cdot>(up\<cdot>0) \<squnion> ae)" by simp
-    also have "\<dots> = Afix2 \<Gamma>\<cdot>(Aexp (App e x)\<cdot>n' \<squnion> ae)" by (rule arg_cong[OF Aexp_App[symmetric]])
+    note IH1 = Application(3)[OF prem3, where n = "inc\<^sub>\<bottom>\<cdot>n", unfolded up Aexp'_simps inc_bot_simps] 
+    note IH2 = Application(5)[OF prem1, where n = n, unfolded up Aexp'_simps]
+    have "Afix \<Theta>\<cdot>(Aexp z\<cdot>n' \<squnion> ae) \<sqsubseteq> Afix \<Delta>\<cdot>(Aexp e'[y::=x]\<cdot>n' \<squnion> ae)" by (rule IH2)
+    also have "\<dots> \<sqsubseteq> Afix \<Delta>\<cdot>(Aexp (App (Lam [y]. e') x)\<cdot>n' \<squnion> ae)" by (intro monofun_cfun_arg monofun_cfun_fun Aexp_subst_App_Lam join_mono below_refl)
+    also have "\<dots> = Afix \<Delta>\<cdot>(Aexp (Lam [y]. e')\<cdot>(inc\<cdot>n') \<squnion> AE_singleton x \<cdot> (up\<cdot>0) \<squnion> ae)"  by (rule arg_cong[OF Aexp_App])
+    also have "\<dots> = Afix \<Delta>\<cdot>(Aexp (Lam [y]. e')\<cdot>(inc\<cdot>n') \<squnion> (AE_singleton x\<cdot>(up\<cdot>0) \<squnion> ae))"  by simp
+    also have "\<dots> \<sqsubseteq> Afix \<Gamma>\<cdot>(Aexp e\<cdot>(inc\<cdot>n') \<squnion> (AE_singleton x\<cdot>(up\<cdot>0) \<squnion> ae))" by (rule IH1)
+    also have "\<dots> = Afix \<Gamma>\<cdot>(Aexp e\<cdot>(inc\<cdot>n') \<squnion> AE_singleton x\<cdot>(up\<cdot>0) \<squnion> ae)" by simp
+    also have "\<dots> = Afix \<Gamma>\<cdot>(Aexp (App e x)\<cdot>n' \<squnion> ae)" by (rule arg_cong[OF Aexp_App[symmetric]])
     finally
     show ?thesis unfolding up by simp
   qed
 next
 case (Let as \<Gamma> L e \<Delta> z ae n)
   hence *: "atom ` domA (asToHeap as) \<sharp>* \<Gamma>" by (metis fresh_star_Pair set_bn_to_atom_domA) 
-  have **: "ae ` domA (asToHeap as) \<subseteq> {\<bottom>}" sorry 
+  note prem = `ae -\` (-{\<bottom>}) \<subseteq> set L`
+  note IH = Let(3)[OF prem]
 
-  have "Afix2 \<Delta>\<cdot>(Aexp' z\<cdot>n \<squnion> ae) \<sqsubseteq> Afix2 (asToHeap as @ \<Gamma>)\<cdot>(Aexp' e\<cdot>n \<squnion> ae)" by (rule Let)
-  also have "\<dots> = Afix2 \<Gamma>\<cdot>(Afix2 (asToHeap as)\<cdot>(Aexp' e\<cdot>n \<squnion> ae))" by (rule Afix2_append_fresh[OF *])
-  also have "\<dots> = Afix2 \<Gamma>\<cdot>(Afix2 (asToHeap as)\<cdot>(Aexp' e\<cdot>n) \<squnion> ae)" by (rule arg_cong[OF Afix2_join_fresh[OF **]])
-  also have "\<dots> \<sqsubseteq> Afix2 \<Gamma>\<cdot>(Aexp' (Let as e)\<cdot>n \<squnion> ae)" by (intro monofun_cfun_arg join_mono below_refl Aexp'_Lam)
+  from `set (bn as) \<sharp>* (\<Gamma>, L)`
+  have "atom ` domA (asToHeap as) \<sharp>* set L" by (auto simp add: fresh_star_Pair set_bn_to_atom_domA fresh_star_set)
+  hence "domA (asToHeap as) \<inter> set L = {}" by (metis Int_commute disjoint_iff_not_equal fresh_list_elem fresh_set fresh_star_def image_eqI not_self_fresh)
+  with prem
+  have **: "ae ` domA (asToHeap as) \<subseteq> {\<bottom>}" by auto 
+
+  have "Afix \<Delta>\<cdot>(Aexp' z\<cdot>n \<squnion> ae) \<sqsubseteq> Afix (asToHeap as @ \<Gamma>)\<cdot>(Aexp' e\<cdot>n \<squnion> ae)" by (rule IH)
+  also have "\<dots> = Afix \<Gamma>\<cdot>(Afix (asToHeap as)\<cdot>(Aexp' e\<cdot>n \<squnion> ae))" by (rule Afix_append_fresh[OF *])
+  also have "\<dots> = Afix \<Gamma>\<cdot>(Afix (asToHeap as)\<cdot>(Aexp' e\<cdot>n) \<squnion> ae)" by (rule arg_cong[OF Afix_join_fresh[OF **]])
+  also have "\<dots> \<sqsubseteq> Afix \<Gamma>\<cdot>(Aexp' (Let as e)\<cdot>n \<squnion> ae)" by (intro monofun_cfun_arg join_mono below_refl Aexp'_Lam)
   finally
-  show "Afix2 \<Delta>\<cdot>(Aexp' z\<cdot>n \<squnion> ae) \<sqsubseteq> Afix2 \<Gamma>\<cdot>(Aexp' (Let as e)\<cdot>n \<squnion> ae)".
+  show "Afix \<Delta>\<cdot>(Aexp' z\<cdot>n \<squnion> ae) \<sqsubseteq> Afix \<Gamma>\<cdot>(Aexp' (Let as e)\<cdot>n \<squnion> ae)".
 qed
 
-(*
-lemma  "\<Gamma> : e \<Down>\<^bsub>L\<^esub> \<Delta> : v \<Longrightarrow> 
-        Afix \<Delta> \<cdot> F \<cdot> (Aexp' v \<cdot> n) \<sqsubseteq> Afix \<Gamma> \<cdot> F \<cdot> (Aexp' e \<cdot> n)"
-proof(induct arbitrary: F n rule: reds.induct)
-case Lambda
-  show ?case by simp
-next
-case (Variable \<Gamma> x e L \<Delta> z F n)
-  have reorder: "map_of ((x, e) # delete x \<Gamma>) = map_of \<Gamma>" by (rule map_of_delete_insert[OF Variable.hyps(1)])
-
-  have "x \<notin> domA \<Delta>" by (rule reds_avoids_live[OF Variable(2), where x = x]) simp_all
-  hence "delete x \<Delta> = \<Delta>" by simp
-
-  note IH =  Variable(3)
-  have "Afix ((x, z) # \<Delta>) \<cdot> F \<cdot>(Aexp' z\<cdot>n) = Afix (delete x \<Delta>) \<cdot> (ABind x z \<squnion> F) \<cdot>(Aexp' z\<cdot>n)" unfolding Afix_bind_to_F..
-  also have "\<dots> = Afix \<Delta> \<cdot> (ABind x z \<squnion> F) \<cdot>(Aexp' z\<cdot>n)" unfolding `delete x \<Delta> = \<Delta>`..
-  also have "\<dots> = Afix \<Delta> \<cdot> ((\<Lambda> ae . Aexp' z \<cdot> (ae x)) \<squnion> F) \<cdot> (Aexp' z\<cdot>n)" unfolding ABind_def..
-  also have "\<dots> = Afix \<Delta> \<cdot> ((\<Lambda> ae . Afix \<Delta> \<cdot> ID \<cdot> (Aexp' z \<cdot> (ae x))) \<squnion> F) \<cdot>(Aexp' z\<cdot>n)" by (rule arg_cong[OF Afix_duplicate_binds]) simp
-  also have "\<dots> \<sqsubseteq> Afix (delete x \<Gamma>) \<cdot> ((\<Lambda> ae. Afix \<Delta> \<cdot> ID \<cdot> (Aexp' z \<cdot> (ae x))) \<squnion> F) \<cdot>(Aexp' e\<cdot>n)"
-    by (rule IH)
-  also have "\<dots> \<sqsubseteq> Afix (delete x \<Gamma>) \<cdot> ((\<Lambda> ae. Afix (delete x \<Gamma>) \<cdot> ID \<cdot> (Aexp' e \<cdot> (ae x))) \<squnion> F) \<cdot>(Aexp' e\<cdot>n)"
-    by (intro monofun_cfun_fun monofun_cfun_arg)(auto intro: IH  join_mono simp add: cfun_below_iff)
-  also have "\<dots> = Afix (delete x \<Gamma>) \<cdot> ((\<Lambda> ae. Aexp' e \<cdot> (ae x)) \<squnion> F)\<cdot>(Aexp' e\<cdot>n)" by (rule arg_cong[OF Afix_duplicate_binds, symmetric]) simp
-  also have "\<dots> = Afix (delete x \<Gamma>) \<cdot> ((ABind x e) \<squnion> F) \<cdot>(Aexp' e\<cdot>n)" unfolding ABind_def..
-  also have "\<dots> = Afix ((x,e) # delete x \<Gamma>) \<cdot> F \<cdot>(Aexp' e\<cdot>n)" unfolding Afix_bind_to_F delete_idem..
-  also have "\<dots> \<sqsubseteq> Afix ((x,e) # delete x \<Gamma>) \<cdot> F \<cdot>(Aexp' (Var x)\<cdot>n)" by (rule Afix_below_var)
-  also have "\<dots> = Afix \<Gamma> \<cdot> F \<cdot>(Aexp' (Var x)\<cdot>n)" by (rule arg_cong[OF Afix_reorder[OF reorder]])
-  finally
-  show "Afix ((x, z) # \<Delta>) \<cdot> F \<cdot>(Aexp' z\<cdot>n) \<sqsubseteq> Afix \<Gamma> \<cdot> F  \<cdot> (Aexp' (Var x)\<cdot>n)".
-next
-case (Application y \<Gamma> e x L \<Delta> \<Theta> z e' F n)
-  show "Afix \<Theta>\<cdot>F\<cdot>(Aexp' z\<cdot>n) \<sqsubseteq> Afix \<Gamma>\<cdot>F\<cdot>(Aexp' (App e x)\<cdot>n)"
-  proof(cases n)
-    case bottom
-    with below_trans[OF Application(5)[where n = "\<bottom>" and F = F, simplified ]  Application(3)[where n = "\<bottom>" and F = F, simplified] ]
-    show ?thesis by (simp add: lambda_strict)
-  next
-    case (up n')
-    note IH = Application(3)[where n = "inc\<^sub>\<bottom>\<cdot>n", unfolded up Aexp'_simps inc_bot_simps] Application(5)[where n = n, unfolded up Aexp'_simps]
-    have "Afix \<Theta>\<cdot>F\<cdot>(Aexp z\<cdot>n') \<sqsubseteq> Afix \<Delta>\<cdot>F\<cdot>(Aexp e'[y::=x]\<cdot>n')" by (rule IH)
-    also have "\<dots> \<sqsubseteq>  Afix \<Delta>\<cdot>F\<cdot>(Aexp (App (Lam [y]. e') x)\<cdot>n')" by (intro monofun_cfun_arg monofun_cfun_fun Aexp_subst_App_Lam)
-    also have "\<dots> =  Afix \<Delta>\<cdot>F\<cdot>(Aexp (Lam [y]. e')\<cdot>(inc\<cdot>n') \<squnion> AE_singleton x (up\<cdot>0))"  by (rule arg_cong[OF Aexp_App])
-    also have "\<dots> =  Afix \<Delta>\<cdot>(F \<squnion> (\<Lambda> _. AE_singleton x (up\<cdot>0)))\<cdot>(Aexp (Lam [y]. e')\<cdot>(inc\<cdot>n'))" unfolding Afix_const_to_F..
-    also have "\<dots> \<sqsubseteq> Afix \<Gamma>\<cdot>(F \<squnion> (\<Lambda> _. AE_singleton x (up\<cdot>0)))\<cdot>(Aexp e\<cdot>(inc\<cdot>n'))" by (rule IH)
-    also have "\<dots> = Afix \<Gamma>\<cdot>F\<cdot>(Aexp e\<cdot>(inc\<cdot>n') \<squnion> AE_singleton x (up\<cdot>0))" unfolding Afix_const_to_F..
-    also have "\<dots> = Afix \<Gamma>\<cdot>F\<cdot>(Aexp (App e x)\<cdot>n')"  by (rule arg_cong[OF Aexp_App[symmetric]])
-    finally
-    show "Afix \<Theta>\<cdot>F\<cdot>(Aexp' z\<cdot>n) \<sqsubseteq> Afix \<Gamma>\<cdot>F\<cdot>(Aexp' (App e x)\<cdot>n)" unfolding up by simp
-  qed
-next
-case (Let as \<Gamma> L e \<Delta> z F n)
-  have "Afix \<Delta>\<cdot>F\<cdot>(Aexp' z\<cdot>n) \<sqsubseteq> Afix (asToHeap as @ \<Gamma>)\<cdot>F\<cdot>(Aexp' e\<cdot>n)" by (rule Let)
-  also have "\<dots> \<sqsubseteq> Afix \<Gamma>\<cdot>F\<cdot>(Aexp' (Terms.Let as e)\<cdot>n)" by (rule Aexp'_Lam)
-  finally
-  show "Afix \<Delta>\<cdot>F\<cdot>(Aexp' z\<cdot>n) \<sqsubseteq> Afix \<Gamma>\<cdot>F\<cdot>(Aexp' (Terms.Let as e)\<cdot>n)".
+corollary  reds_improves_arity:
+ assumes "\<Gamma> : e \<Down>\<^bsub>L\<^esub> \<Delta> : v"
+  shows "Afix \<Delta> \<cdot> (Aexp' v \<cdot> n) \<sqsubseteq> Afix \<Gamma> \<cdot> (Aexp' e \<cdot> n)"
+proof-
+  have simp: "\<bottom> -` (- {\<bottom>}) = {}" by auto
+  show ?thesis by (rule reds_improves_arity'[where ae = \<bottom>, OF assms, simplified]) auto
 qed
-*)
-
 end
+
+unused_thms
 
 end
